$$
X\in R^{N\times D_{in}}\\
Y\in R^{N\times D_{out}}\\
W_1\in R^{D_{in}\times H}\\
W_2\in R^{H\times D_{out}}\\
H=XW_1\\
H_{relu}=max(H,0)\\
Y_{pred}=H_{relu}W_2\\
loss=||Y_{pred}-Y||_F^{2}\\
$$

$$
1.求\frac{\part{loss}}{\part{Y_{pred}}}\\
因为d(loss)=d(||Y_{pred}-Y||_F^{2})=tr(2(Y_{pred}-Y)^{\top}dY_{pred})\\
所以\frac{\part{loss}}{\part{Y_{pred}}}=2(Y_{pred}-Y)\\
$$

$$
2.求\frac{\part{loss}}{\part{W_2}}\\
因为d(loss)=d(||Y_{pred}-Y||_F^{2})\\
=d(||H_{relu}W_2-Y||_F^2)\\
=tr(2(H_{relu}W_2-Y)^{\top}d(H_{relu}W_2-Y))\\
=tr(2(H_{relu}W_2-Y)^{\top}dH_{relu}W_2)\\
=tr(2(H_{relu}W_2-Y)^{\top}H_{relu}dW_2)\\
所以\frac{\part{loss}}{\part{H_{relu}}}=2H_{relu}^{\top}(H_{relu}W_2-Y)\\
=H_{relu}^{\top}\frac{\part{loss}}{\part{Y_{pred}}}
$$

$$
3.求\frac{\part{loss}}{\part{H_{relu}}}\\
因为d(loss)=d(||Y_{pred}-Y||_F^{2})\\
=d(||H_{relu}W_2-Y||_F^2)\\
=tr(2(H_{relu}W_2-Y)^{\top}d(H_{relu}W_2-Y))\\
=tr(2(H_{relu}W_2-Y)^{\top}dH_{relu}W_2)\\
=tr(2W_2(H_{relu}W_2-Y)^{\top}dH_{relu})\\
所以\frac{\part{loss}}{\part{H_{relu}}}=2(H_{relu}W_2-Y)W_2^{\top}\\
=\frac{\part{loss}}{\part{Y_{pred}}}W_{2}^{\top}
$$

$$
4.求\frac{\part{loss}}{\part{H}}\\
因为d(loss)=tr(2W_2(H_{relu}W_2-Y)^{\top}dH_{relu})\\
且H_{relu}=max(H,0)\\
若H>0，H_{relu}=H，d(loss)=tr(2W_2(H_{relu}W_2-Y)^{\top}dH)\\
\frac{\part{loss}}{\part{H}}=2(H_{relu}W_2-Y)W_2^{\top}=\frac{\part{loss}}{\part{H_{relu}}}\\
若H<=0，H_{relu}=0,d(loss)=0\\
\frac{\part{loss}}{\part{H}}=0
$$

$$
5.求\frac{\part{loss}}{\part{W_1}}\\
因为d(loss)=tr(2W_2(H_{relu}W_2-Y)^{\top}dH)\\
=tr(2W_2(H_{relu}W_2-Y)^{\top}dXW_1)\\
=tr(2W_2(H_{relu}W_2-Y)^{\top}XdW_1)\\
所以\frac{\part{loss}}{\part{W_1}}=X^{\top}2(H_{relu}W_2-Y)W_2^{\top}=X^{\top}\frac{\part{loss}}{\part{H}}
$$



